Wavelet/Compile/Fn/Simulation.lean
@@ -1,20 +1,66 @@
 import Wavelet.Compile.Fn.Defs
 
+import Wavelet.Compile.Fn.Simulation.Invariants
+import Wavelet.Compile.Fn.Simulation.Init
+import Wavelet.Compile.Fn.Simulation.Ret
+import Wavelet.Compile.Fn.Simulation.Tail
+import Wavelet.Compile.Fn.Simulation.Op
+import Wavelet.Compile.Fn.Simulation.Br
+
 /-! Simulation proofs for `compileFn`. -/
 
 namespace Wavelet.Compile
 
-open Semantics Seq Dataflow
+open Semantics Seq Dataflow Fn
 
-/-- TODO: Migrate the proofs of the older version over. -/
+private theorem sim_compile_fn_init
+  [Arity Op]
+  [InterpConsts V]
+  [DecidableEq χ]
+  (fn : Fn Op χ V m n)
+  (hnz : m > 0 ∧ n > 0)
+  (hwf : fn.WellFormed) :
+  SimRel hnz fn.semantics.init (compileFn hnz fn).semantics.init
+  := by
+  simp [semantics, Fn.semantics, Seq.Config.init,
+    Proc.semantics, Dataflow.Config.init]
+  and_intros
+  · simp
+    funext name
+    simp [ChanMap.empty, varsToChans, VarMap.getVar, VarMap.empty]
+    cases name <;> rfl
+  · simp
+  · simp [VarMap.empty, VarMap.getVar]
+  · simp [OrderedPathConds]
+  · simp
+  · simp [HasMerges]
+  · exact hwf.1
+  · exact hwf.2
+  · simp [compileFn, compileFn.inputs]
+  · simp [compileFn, compileFn.outputs]
+  · simp [HasCompiledProcs, compileFn]
+
+/-- Main forward simulation result for `compileFn`. -/
 theorem sim_compile_fn
   [Arity Op]
   [InterpConsts V]
   [DecidableEq χ]
-  (hnz : m > 0 ∧ n > 0)
   (fn : Fn Op χ V m n)
+  (hnz : m > 0 ∧ n > 0)
   (hwf : fn.WellFormed) :
   fn.semantics ≲ (compileFn hnz fn).semantics
-  := sorry
+  := by
+  apply Lts.SimilarBy.mk (SimRel hnz)
+  apply Semantics.SimulatedBy.alt
+  · exact sim_compile_fn_init fn hnz hwf
+  · intros ec pc l ec' hsim hstep
+    cases h₁ : ec.cont with
+    | init => exact sim_step_init hsim hstep h₁
+    | expr expr =>
+      cases h₂ : expr <;> simp [h₂] at h₁
+      case ret => exact sim_step_ret hsim hstep h₁
+      case tail => exact sim_step_tail hsim hstep h₁
+      case op => exact sim_step_op hsim hstep h₁
+      case br => exact sim_step_br hsim hstep h₁
 
 end Wavelet.Compile
