Wavelet/Compile/Fn/Simulation/Tail.lean
@@ -1,0 +1,522 @@
+import Mathlib.Data.List.Basic
+import Mathlib.Data.List.Nodup
+import Mathlib.Logic.Relation
+import Batteries.Data.Vector.Lemmas
+
+import Wavelet.Compile.Fn.Defs
+import Wavelet.Compile.Fn.Simulation.Invariants
+import Wavelet.Compile.Fn.Simulation.BrMerges
+import Wavelet.Compile.Fn.Lemmas
+
+/-! Simulation in the case of tail call. -/
+
+namespace Wavelet.Compile.Fn
+
+open Semantics Seq Dataflow Compile Fn
+
+/-- Values pushed to output channels in the case of a tail call. -/
+private def tailArgsToExprOutputs
+  [InterpConsts V]
+  (tailArgs : Vector V m) : Vector V (n + (m + 1)) :=
+  Vector.replicate n (InterpConsts.junkVal : V) ++
+  tailArgs.push (InterpConsts.fromBool true)
+
+/-- Fires `forwardc` and `sink` to get an intermediate state. -/
+private theorem sim_step_tail_forwardc_sink
+  [Arity Op] [InterpConsts V] [DecidableEq χ]
+  {ec : Seq.Config Op χ V m n}
+  {pc : Dataflow.Config Op (ChanName χ) V m n}
+  {hnz : m > 0 ∧ n > 0}
+  (hsim : SimRel hnz ec pc)
+  (hexpr : ec.cont = .expr (.tail vars))
+  (hvars : VarMap.getVars vars ec.vars = some tailArgs)
+  (hvars_nodup : vars.toList.Nodup) :
+  Dataflow.Config.Step.StepModTau .τ pc .τ
+  { proc := pc.proc,
+    chans := intermChans ec pc vars
+      (tailArgsToExprOutputs tailArgs)
+      ec.pathConds }
+:= by
+  have ⟨
+    rest, carryInLoop, ctxLeft, ctxCurrent, ctxRight,
+    hatoms, hcomp_fn, hrest, hret, hcont,
+  ⟩ := hsim.has_compiled_procs
+  have ⟨hcarryInLoop, hwf_expr, hcurrent⟩ := hcont _ hexpr
+  simp [compileExpr] at hcurrent
+  -- Step 1: Fire `forwardc`.
+  have ⟨chans₁, tailArgs', hpop_tail_args, hchans₁, htail_args⟩ :=
+    pop_vals_singleton _ _
+    (map := pc.chans)
+    (names := vars.map (.var · ec.pathConds))
+    (λ name val =>
+      ∃ var,
+        name = .var var ec.pathConds ∧
+        ec.vars.getVar var = some val)
+    (by
+      simp only [Vector.toList_map]
+      apply List.Nodup.map _ hvars_nodup
+      simp [Function.Injective])
+    (by
+      simp [hsim.vars_to_chans, varsToChans]
+      have := Vector.mapM_some_implies_all_some hvars
+      intros v hmem_v
+      have ⟨val, _, hval⟩ := this v hmem_v
+      exists val
+      simp [VarMap.getVar, hval])
+  have heq_ret_vals :
+    tailArgs' = tailArgs
+  := by
+    apply Vector.toList_inj.mp
+    apply List.right_unique_forall₂' _ htail_args
+    · simp [Vector.toList_map, VarMap.getVar]
+      apply List.mapM_some_iff_forall₂.mp (Vector.mapM_toList hvars)
+    · simp only [Relator.RightUnique]
+      intros a b c hb hc
+      have ⟨_, hb₁, hb₂⟩ := hb
+      have ⟨_, hc₁, hc₂⟩ := hc
+      simp [hb₁] at hc₁
+      subst hc₁
+      simp [hb₂] at hc₂
+      exact hc₂
+  replace heq_ret_vals := heq_ret_vals.symm
+  subst heq_ret_vals
+  have hmem_forwardc :
+    AtomicProc.forwardc
+      (vars.map (.var · ec.pathConds))
+      ((Vector.replicate n InterpConsts.junkVal).push (InterpConsts.fromBool true))
+      (compileExpr.tailExprOutputs m n ec.pathConds)
+      ∈ pc.proc.atoms
+  := by grind
+  have hsteps₁ : Dataflow.Config.Step.StepModTau .τ pc _ _
+    := .single (Dataflow.Config.Step.step_forwardc hmem_forwardc hpop_tail_args)
+  -- Simplify pushes
+  rw [push_vals_empty] at hsteps₁
+  rotate_left
+  · apply tailExprOutputs_nodup
+  · intros name hmem_name
+    simp at hmem_name
+    simp [hchans₁, hsim.vars_to_chans, varsToChans]
+    simp [compileExpr.tailExprOutputs] at hmem_name
+    rcases hmem_name with ⟨_, _, h⟩ | ⟨_, _, h⟩ | h
+    · simp [← h]
+    · simp [← h]
+    · simp [h]
+  simp only [hchans₁] at hsteps₁
+  replace ⟨pc₁, hpc₁, hsteps₁⟩ := exists_eq_left.mpr hsteps₁
+  -- Step 2: Fire `sink` to consume all unused channels in the current context.
+  have ⟨chans₂, otherVals, hpop_other_vals, hchans₂, hother_vals⟩ :=
+    pop_vals_singleton _ _
+    (map := pc₁.chans)
+    (names := compileExpr.allVarsExcept ec.definedVars vars.toList ec.pathConds)
+    (λ name val => True)
+    (allVarsExcept_nodup hsim.defined_vars_nodup)
+    (by
+      simp
+      intros name hname
+      have ⟨var, hvar, hmem_var, hnot_mem_var⟩ := mem_allVarsExcept hname
+      simp [hvar, hpc₁]
+      simp [hsim.vars_to_chans, varsToChans]
+      have ⟨val, h⟩ := hsim.defined_vars_to_get_var hmem_var
+      exists val
+      simp at hnot_mem_var
+      simp [h, hnot_mem_var])
+  have hmem_sink :
+    .sink (compileExpr.allVarsExcept ec.definedVars vars.toList ec.pathConds)
+    ∈ pc₁.proc.atoms
+  := by grind
+  have hsteps₂ : Dataflow.Config.Step.StepModTau .τ pc _ _
+    := .tail_tau hsteps₁
+      (Dataflow.Config.Step.step_sink hmem_sink hpop_other_vals)
+  apply hsteps₂.eq_rhs
+  simp [hpc₁]
+  funext name
+  simp [intermChans, hchans₂, hpc₁]
+  split <;> rename_i h₁
+  · have ⟨var, hvar, hmem_var, hnot_mem_var⟩ := mem_allVarsExcept h₁
+    simp [hvar]
+  · split <;> rename_i h₂
+    · simp [tailExprOutputs_finIdxOf?_some_to_exprOutputs h₂, tailArgsToExprOutputs]
+      -- Rearrange positions of tail arguments and return values
+      rename_i i
+      split_ifs <;> rename_i h₃
+      · simp [h₃]
+      · rename_i h₄
+        have : ↑i - m < n := by omega
+        simp [Vector.getElem_push, Vector.getElem_append]
+        simp [h₄, this]
+      · rename_i h₄
+        simp at h₃
+        simp [Vector.getElem_push, Vector.getElem_append]
+        have h₅ : ↑i ≥ m := by omega
+        have h₆ : ↑i - m ≥ n := by omega
+        simp [h₄, h₆]
+    · have := Option.eq_none_iff_forall_ne_some.mpr h₂
+      have := tailExprOutputs_finIdxOf?_none_to_exprOutputs this
+      simp [this]
+      split <;> rename_i h₃
+      · rfl
+      · simp [hsim.vars_to_chans, varsToChans]
+        cases name with
+        | var var' pathConds' =>
+          simp
+          intros h
+          simp [h] at h₃
+          simp [compileExpr.allVarsExcept, List.toVector] at h₁
+          split <;> rename_i h₄
+          · replace h₄ := hsim.get_var_to_defined_vars ⟨_, h₄⟩
+            have := h₁ (List.mem_to_mem_removeAll h₄ (by simp [h₃]))
+            simp [h] at this
+          · rfl
+        | _ => rfl
+
+/- TODO: Fix proof performance -/
+set_option maxHeartbeats 300000
+
+/-- Fires relevant operators on the dataflow side. -/
+private theorem sim_step_tail_exec_dataflow
+  [Arity Op] [InterpConsts V] [DecidableEq χ]
+  {l : Label Op V m n}
+  {ec ec' : Seq.Config Op χ V m n}
+  {pc : Dataflow.Config Op (ChanName χ) V m n}
+  {hnz : m > 0 ∧ n > 0}
+  (hsim : SimRel hnz ec pc)
+  (hstep : Config.Step ec l ec')
+  (hexpr : ec.cont = .expr (.tail vars)) :
+  Dataflow.Config.Step.StepModTau .τ pc l {
+    proc := pc.proc,
+    chans := varsToChans ec',
+  }
+:= by
+  have ⟨
+    rest, carryInLoop, ctxLeft, ctxCurrent, ctxRight,
+    hatoms, hcomp_fn, hrest, hret, hcont,
+  ⟩ := hsim.has_compiled_procs
+  have ⟨hcarryInLoop, hwf_expr, hcurrent⟩ := hcont _ hexpr
+  cases hstep with
+  | step_init hexpr' | step_br hexpr' | step_ret hexpr' | step_op hexpr' =>
+    simp [hexpr] at hexpr'
+  | step_tail hexpr' hvars =>
+  rename_i tailArgs vars'
+  simp [hexpr] at hexpr'
+  subst hexpr'
+  cases hwf_expr with | wf_tail hvars_nodup =>
+  -- Step 1: Fire `forwardc` and `sink`
+  have hsteps₁ := sim_step_tail_forwardc_sink hsim hexpr hvars hvars_nodup
+  -- Step 2: Fire final merges
+  have hsteps₂ := sim_step_merges ec pc
+    hsim.has_merges (by simp)
+    hsim.path_conds_nodup hsteps₁
+  -- Step 3: Fire the `fork` in `compileFn`.
+  simp [compileFn, compileFn.resultSteers] at hcomp_fn
+  have ⟨chans₁, hpop_tail_cond, hchans₁⟩ := pop_val_singleton _ _
+    (map := intermChans ec pc vars
+      (tailArgsToExprOutputs tailArgs)
+      [])
+    (name := .tail_cond [])
+    (val := InterpConsts.fromBool true)
+    (by simp [intermChans, exprOutputs_finIdxOf?_tail_cond, tailArgsToExprOutputs])
+  have hmem_fork :
+    .fork (ChanName.tail_cond [])
+      #v[.tail_cond_carry, .tail_cond_steer_dests, .tail_cond_steer_tail_args]
+    ∈ pc.proc.atoms
+  := by simp [hatoms, ← hcomp_fn]
+  have hsteps₃ : Dataflow.Config.Step.StepModTau .τ pc _ _
+    := .tail_tau hsteps₂
+      (Dataflow.Config.Step.step_fork hmem_fork hpop_tail_cond)
+  -- Simplify pushes
+  rw [push_vals_empty] at hsteps₃
+  rotate_left
+  · simp
+  · simp [hchans₁, intermChans]
+  simp at hsteps₃
+  replace ⟨pc₁, hpc₁, hsteps₃⟩ := exists_eq_left.mpr hsteps₃
+  -- Step 4: Fire the first `steer` in `compileFn` for return values.
+  have ⟨chans₂, hpop_tail_cond_steer_dests, hchans₂⟩ := pop_val_singleton _ _
+    (map := pc₁.chans)
+    (name := .tail_cond_steer_dests)
+    (val := InterpConsts.fromBool true)
+    (by simp [hpc₁, List.finIdxOf?, List.findFinIdx?, List.findFinIdx?.go])
+  have ⟨chans₃, retVals, hpop_ret_vals, hchans₃, hret_vals⟩ :=
+    pop_vals_singleton _ _
+    (map := chans₂)
+    (names := (Vector.range n).map (.dest · []))
+    (λ name val => True)
+    (by
+      simp [Vector.toList_map, Vector.toList_range]
+      apply List.Nodup.map _ List.nodup_range
+      simp [Function.Injective])
+    (by
+      intros name hname
+      simp at hname
+      replace ⟨i, h₂, hname⟩ := hname
+      simp [← hname, hchans₂, hpc₁, hchans₁, intermChans,
+        List.finIdxOf?, List.findFinIdx?, List.findFinIdx?.go,
+        exprOutputs_finIdxOf?_dest h₂, h₂, tailArgsToExprOutputs])
+  have hmem_steer_dests :
+    .steer false
+      .tail_cond_steer_dests
+      ((Vector.range n).map (.dest · []))
+      ((Vector.range n).map .final_dest)
+    ∈ pc₁.proc.atoms
+  := by simp [hpc₁, hatoms, ← hcomp_fn]
+  have hsteps₄ : Dataflow.Config.Step.StepModTau .τ pc _ _
+    := .tail_tau hsteps₃
+      (Dataflow.Config.Step.step_steer
+        hmem_steer_dests
+        hpop_tail_cond_steer_dests
+        hpop_ret_vals
+        (InterpConsts.unique_fromBool_toBool _))
+  -- Simplify pushes
+  rw [push_vals_empty] at hsteps₄
+  rotate_left
+  · simp [Vector.toList_map, Vector.toList_range]
+    apply List.Nodup.map _ List.nodup_range
+    simp [Function.Injective]
+  · simp [hchans₃, hchans₂, hpc₁,
+      List.finIdxOf?, List.findFinIdx?, List.findFinIdx?.go,
+      hchans₁, intermChans]
+  simp at hsteps₄
+  replace ⟨pc₂, hpc₂, hsteps₄⟩ := exists_eq_left.mpr hsteps₄
+  -- Step 5: Fire the second `steer` in `compileFn` for tail call args.
+  have ⟨chans₄, hpop_tail_cond_steer_tail_args, hchans₄⟩ := pop_val_singleton _ _
+    (map := pc₂.chans)
+    (name := .tail_cond_steer_tail_args)
+    (val := InterpConsts.fromBool true)
+    (by
+      simp [hpc₂, hchans₃, hchans₂, hpc₁,
+        List.finIdxOf?, List.findFinIdx?, List.findFinIdx?.go])
+  have ⟨chans₅, tailArgVals, hpop_tail_arg_vals, hchans₅, htail_arg_vals⟩ :=
+    pop_vals_singleton _ _
+    (map := chans₄)
+    (names := (Vector.range m).map (.tail_arg · []))
+    (λ name val =>
+      match name with
+      | .tail_arg i _ => ∃ (h : i < m), val = tailArgs[i]
+      | _ => False)
+    (by
+      simp [Vector.toList_map, Vector.toList_range]
+      apply List.Nodup.map _ List.nodup_range
+      simp [Function.Injective])
+    (by
+      simp
+      intros i hi
+      simp [hchans₄, hpc₂, hchans₃, hchans₂, hpc₁,
+        List.finIdxOf?, List.findFinIdx?, List.findFinIdx?.go,
+        hchans₁, intermChans, tailArgsToExprOutputs,
+        exprOutputs_finIdxOf?_tail_args hi, hi])
+  have : tailArgs = tailArgVals := by
+    symm
+    apply Vector.toList_inj.mp
+    apply List.right_unique_forall₂' _ htail_arg_vals
+    · apply List.forall₂_iff_get.mpr
+      simp [Vector.toList_map, Vector.toList_range]
+    · simp [Relator.RightUnique]
+      intros a b c hb hc
+      split at hb <;> simp at hc
+      replace ⟨_, hb⟩ := hb
+      replace ⟨_, hc⟩ := hc
+      simp [hc, hb]
+  subst this
+  have hmem_steer_tail_args :
+    .steer true
+      .tail_cond_steer_tail_args
+      ((Vector.range m).map (.tail_arg · []))
+      ((Vector.range m).map .final_tail_arg)
+    ∈ pc₂.proc.atoms
+  := by simp [hpc₂, hpc₁, hatoms, ← hcomp_fn]
+  have hsteps₅ : Dataflow.Config.Step.StepModTau .τ pc _ _
+    := .tail_tau hsteps₄
+      (Dataflow.Config.Step.step_steer
+        hmem_steer_tail_args
+        hpop_tail_cond_steer_tail_args
+        hpop_tail_arg_vals
+        (InterpConsts.unique_fromBool_toBool _))
+  rw [push_vals_empty] at hsteps₅
+  rotate_left
+  · simp [Vector.toList_map, Vector.toList_range]
+    apply List.Nodup.map _ List.nodup_range
+    simp [Function.Injective]
+  · simp [hchans₅, hchans₄, hpc₂, hchans₃, hchans₂, hpc₁,
+      List.finIdxOf?, List.findFinIdx?, List.findFinIdx?.go,
+      hchans₁, intermChans]
+  simp at hsteps₅
+  replace ⟨pc₃, hpc₃, hsteps₅⟩ := exists_eq_left.mpr hsteps₅
+  -- Step 6: Fire the first `carry` in `compileFn`.
+  have ⟨chans₆, hpop_tail_cond_steer_tail_args, hchans₆⟩ := pop_val_singleton _ _
+    (map := pc₃.chans)
+    (name := .tail_cond_carry)
+    (val := InterpConsts.fromBool true)
+    (by simp [hpc₃, hchans₅, hchans₄, hpc₂, hchans₃, hchans₂, hpc₁,
+      List.finIdxOf?, List.findFinIdx?, List.findFinIdx?.go])
+  have ⟨chans₇, tailArgs', hpop_final_tail_args, hchans₇, hfinal_tail_args⟩ :=
+    pop_vals_singleton _ _
+    (map := chans₆)
+    (names := (Vector.range m).map .final_tail_arg)
+    (λ name val =>
+      match name with
+      | .final_tail_arg i => ∃ (h : i < m), val = tailArgs[i]
+      | _ => False)
+    (by
+      simp [Vector.toList_map, Vector.toList_range]
+      apply List.Nodup.map _ List.nodup_range
+      simp [Function.Injective])
+    (by
+      simp
+      intros i hi
+      simp [hchans₆, hpc₃]
+      split <;> rename_i h₁
+      · simp at h₁
+        simp
+        exists hi
+        congr 1
+        omega
+      · have := Option.eq_none_iff_forall_ne_some.mpr h₁
+        simp at this
+        omega)
+  have : tailArgs = tailArgs' := by
+    symm
+    apply Vector.toList_inj.mp
+    apply List.right_unique_forall₂' _ hfinal_tail_args
+    · simp [Vector.toList_map, Vector.toList_range]
+      apply List.forall₂_iff_get.mpr
+      simp
+    · simp [Relator.RightUnique]
+      intros a b c hb hc
+      split at hb <;> simp at hc
+      replace ⟨_, hb⟩ := hb
+      replace ⟨_, hc⟩ := hc
+      simp [hc, hb]
+  subst this
+  have hmem_carry :
+    pc₃.proc.atoms = [] ++ [compileFn.initCarry ec.fn carryInLoop] ++ rest
+  := by simp [hpc₃, hpc₂, hpc₁, hatoms]
+  simp only [compileFn.initCarry, hcarryInLoop] at hmem_carry
+  have hsteps₆ : Dataflow.Config.Step.StepModTau .τ pc _ _
+    := .tail_tau hsteps₅
+      (Dataflow.Config.Step.step_carry_true
+        hmem_carry
+        hpop_tail_cond_steer_tail_args
+        (InterpConsts.unique_fromBool_toBool _)
+        hpop_final_tail_args)
+  -- Simplify pushes
+  rw [push_vals_empty] at hsteps₆
+  rotate_left
+  · simp [Vector.toList_map]
+    apply List.Nodup.map _ hsim.wf_fn.1
+    simp [Function.Injective]
+  · intros name hname
+    simp at hname
+    have ⟨var, hmem_var, hname⟩ := hname
+    simp [← hname, hchans₇, hchans₆, hpc₃, hchans₅, hchans₄, hpc₂,
+      hchans₃, hchans₂, hpc₁,
+      List.finIdxOf?, List.findFinIdx?, List.findFinIdx?.go,
+      hchans₁, intermChans]
+  simp at hsteps₆
+  replace ⟨pc', hpc', hsteps₆⟩ := exists_eq_left.mpr hsteps₆
+  apply hsteps₆.eq_rhs
+  simp [hpc', hpc₃, hpc₂, hpc₁,
+    hchans₇, hchans₆, hchans₅, hchans₄, hchans₃, hchans₂, hchans₁,
+    List.finIdxOf?, List.findFinIdx?, List.findFinIdx?.go, intermChans]
+  -- Prove that the final channel maps match
+  funext name
+  simp [varsToChans]
+  cases name with
+  | var v pathConds =>
+    simp
+    if h₁ : pathConds = [] then
+      simp [h₁]
+      split <;> rename_i h₂
+      · rename_i i
+        simp at h₂
+        simp [Vector.get] at h₂
+        simp [← h₂.1]
+        simp [var_map_fromList_get_vars_index hsim.wf_fn.1]
+      · have := Option.eq_none_iff_forall_ne_some.mpr h₂
+        simp at this
+        simp
+        split <;> rename_i h₃
+        · have h₄ := var_map_fromList_get_vars.mpr ⟨_, h₃⟩
+          exact False.elim (this h₄)
+        · rfl
+    else
+      simp [h₁]
+  | dest =>
+    simp
+    intros h₁
+    simp [exprOutputs_finIdxOf?_no_match_dest h₁]
+  | tail_arg =>
+    simp
+    intros h₁
+    simp [exprOutputs_finIdxOf?_no_match_tail_args h₁]
+  | tail_cond =>
+    simp
+    intros h₁
+    simp [exprOutputs_finIdxOf?_no_match_tail_cond h₁]
+  | final_tail_arg =>
+    simp
+    split <;> rename_i h₁
+    · simp at h₁
+      omega
+    · simp
+  | input | switch_cond | merge_cond
+  | tail_cond_carry | tail_cond_steer_dests | tail_cond_steer_tail_args
+  | final_dest =>
+    simp
+
+/-- TODO: these theorems are similar to `sim_step_ret`,
+figure out a way to share these proofs. -/
+theorem sim_step_tail
+  [Arity Op] [InterpConsts V] [DecidableEq χ]
+  {l : Label Op V m n}
+  {ec ec' : Seq.Config Op χ V m n}
+  {pc : Dataflow.Config Op (ChanName χ) V m n}
+  {hnz : m > 0 ∧ n > 0}
+  (hsim : SimRel hnz ec pc)
+  (hstep : Config.Step ec l ec')
+  (hexpr : ec.cont = .expr (.tail vars)) :
+  ∃ pc',
+    Config.Step.StepModTau .τ pc l pc' ∧
+    SimRel hnz ec' pc' := by
+  have hsteps := sim_step_tail_exec_dataflow hsim hstep hexpr
+  replace ⟨pc', hpc', hsteps⟩ := exists_eq_left.mpr hsteps
+  have ⟨
+    rest, carryInLoop, ctxLeft, ctxCurrent, ctxRight,
+    hatoms, hcomp_fn, hrest, hret, hcont,
+  ⟩ := hsim.has_compiled_procs
+  have ⟨hcarryInLoop, hwf_expr, hcurrent⟩ := hcont _ hexpr
+  cases hstep with
+  | step_init hexpr' | step_br hexpr' | step_ret hexpr' | step_op hexpr' =>
+    simp [hexpr] at hexpr'
+  | step_tail hexpr' hvars =>
+    rename_i tailArgs vars'
+    simp [hexpr] at hexpr'
+    subst hexpr'
+    cases hwf_expr with | wf_tail hvars_nodup =>
+    exists pc'
+    constructor
+    · exact hsteps
+    · simp only [hpc']
+      and_intros
+      · simp
+      · simp [hsim.wf_fn.1]
+      · simp []
+        intros var
+        apply var_map_fromList_get_vars
+      · simp [OrderedPathConds]
+      · simp
+      · simp [HasMerges]
+      · exact hsim.wf_fn.1
+      · exact hsim.wf_fn.2
+      · exact hsim.inputs
+      · exact hsim.outputs
+      · simp [compileFn.initCarry, HasCompiledProcs]
+        exists rest
+        simp [hatoms, compileFn, compileFn.initCarry, hcarryInLoop]
+        simp [compileFn] at hcomp_fn
+        simp [hcomp_fn]
+        constructor
+        · exists [], compileFn.resultSteers m n
+          simp [← hcomp_fn, compileFn.bodyComp]
+        · exact hsim.wf_fn.2
+
+end Wavelet.Compile.Fn
